Finish the (TAPPLY) case in preservation

CC/Subtype/Inversion.lean
@@ -216,3 +216,75 @@ lemma SubtypeP.tfun_inv :
   (∃ T' U', P = PType.tarr T' U' ∧ SubtypeP Γ T T' ∧ Subtype (Ctx.extend_tvar Γ T) U' U) := by
   intro h
   apply SubtypeP.tfun_inv' <;> aesop
+
+private def SubtypeP.boxed_inv_motive (Γ : Ctx n m) (S1 S2 : PType n m) : Prop :=
+  ∀ T, 
+    S2 = PType.boxed T ->
+    SubtypeP Γ S1 S2 ->
+    (∃ X, S1 = PType.tvar X) ∨ 
+    (∃ T', S1 = PType.boxed T' ∧ Subtype Γ T' T)
+
+lemma SubtypeP.boxed_inv'
+  (h : SubtypeP Γ S1 S2) :
+  SubtypeP.boxed_inv_motive Γ S1 S2 := by
+  apply SubtypeP.rec
+    (motive_1 := fun Γ T1 T2 _ => True)
+    (motive_2 := fun Γ S1 S2 _ => SubtypeP.boxed_inv_motive Γ S1 S2)
+    <;> try (solve | trivial | intros; trivial | intros; unfold boxed_inv_motive; intros _ he; cases he)
+  case refl =>
+    intros; unfold boxed_inv_motive
+    intros
+    apply Or.inr
+    repeat apply Exists.intro
+    constructor
+    trivial
+    apply Subtype.refl
+  case trans =>
+    intros; unfold boxed_inv_motive at *
+    intros T he h
+    rename_i h1 h2 ih1 ih2
+    subst_vars
+    have ih2' := ih2 _ rfl h2
+    cases ih2'
+    case inl ih =>
+      let ⟨X0, he0⟩ := ih
+      subst_vars
+      have h1' := SubtypeP.tvar_inv h1
+      aesop
+    case inr ih =>
+      let ⟨T', he, ih1⟩ := ih
+      subst_vars
+      have ih' := ih1 _ rfl h1
+      cases ih'
+      case inl => aesop
+      case inr ih' =>
+        let ⟨T'', he', ih1'⟩ := ih'
+        subst_vars
+        apply Or.inr
+        repeat apply Exists.intro
+        constructor
+        trivial
+        apply Subtype.trans <;> trivial
+  case tvar =>
+    intros; unfold boxed_inv_motive at *
+    intros T he h
+    subst_vars
+    apply Or.inl
+    apply Exists.intro
+    rfl
+  case boxed =>
+    intros; unfold boxed_inv_motive at *
+    intros T he h
+    subst_vars
+    apply Or.inr
+    repeat apply Exists.intro
+    constructor
+    trivial
+    aesop
+
+lemma SubtypeP.boxed_inv :
+  SubtypeP Γ P (PType.boxed T) ->
+  (∃ X, P = PType.tvar X) ∨ 
+  (∃ T', P = PType.boxed T' ∧ Subtype Γ T' T) := by
+  intro h
+  apply SubtypeP.boxed_inv' <;> aesop
