CC/Opening.lean
@@ -1,0 +1,44 @@
+import Mathlib.Data.Finset.Basic
+import Mathlib.Data.Finset.Image
+
+import CC.Basic
+import CC.Rename
+
+import CC.CaptureSet
+import CC.Context
+import CC.Type
+import CC.Subcapt
+import CC.Subcapt.Basic
+import CC.Subcapt.Rename
+import CC.Subtype
+import CC.Subtype.Rename
+import CC.Subtype.Basic
+import CC.Subst
+import CC.TypeMap
+import CC.Type.TypeSubst
+
+namespace CC
+
+def VarTypeMap.open_tvar :
+  VarTypeMap (Ctx.extend_tvar Γ S) Γ (tvar_open_map S') := by
+  intros x T h
+  cases h with
+  | there_tvar h =>
+    rw [<- CType.open_tvar_def]
+    simp [CType.open_tvar_weaken_tvar_id]
+    trivial
+
+def TVarSubst.open_tvar
+  (hsub : SubtypeP Γ S' S) :
+  TVarSubst (Ctx.extend_tvar Γ S) Γ (tvar_open_map S') := by
+  intros X P h
+  cases h with
+  | here =>
+    rw [<- PType.open_tvar_def]
+    simp [PType.open_tvar_weaken_tvar_id]
+    trivial
+  | there_tvar =>
+    rw [<- PType.open_tvar_def]
+    simp [PType.open_tvar_weaken_tvar_id, tvar_open_map]
+    apply SubtypeP.tvar
+    trivial
