CC/Typed/Opening.lean
@@ -1,0 +1,32 @@
+import Mathlib.Data.Finset.Basic
+import Mathlib.Data.Finset.Image
+
+import CC.Basic
+import CC.Rename
+
+import CC.CaptureSet
+import CC.Context
+import CC.Type
+import CC.Term.TypeSubst
+import CC.Subcapt
+import CC.Subcapt.Basic
+import CC.Subcapt.Rename
+import CC.Subtype
+import CC.Subtype.Rename
+import CC.Subtype.Basic
+import CC.Subst
+import CC.TypeMap
+import CC.Type.TypeSubst
+import CC.Typed.TypeSubst
+import CC.Opening
+
+namespace CC
+
+def Typed.open_tvar
+  (hsub : SubtypeP Γ S' S)
+  (h0 : Typed (Ctx.extend_tvar Γ S) t Ct T) :
+  Typed Γ (t.open_tvar S') Ct (T.open_tvar S') := by
+  unfold Term.open_tvar; unfold CType.open_tvar
+  apply Typed.tsubst h0
+  apply VarTypeMap.open_tvar
+  apply TVarSubst.open_tvar; trivial
